src/tls/TLS.Handshake.fst
@@ -14,13 +14,16 @@ open TLSConstants
 open Range
 open Old.Epochs
 
+open TLS.Handshake.Client
+open TLS.Handshake.Server
+
 module U32 = FStar.UInt32
 module MS = FStar.Monotonic.Seq
 module HS = FStar.HyperStack
 module Nego = Negotiation
 module HST = FStar.HyperStack.ST
 module Epochs = Old.Epochs
-module KeySchedule = Old.KeySchedule
+module KS = Old.KeySchedule
 module HMAC_UFCMA = Old.HMAC.UFCMA
 module HSM = HandshakeMessages
 module HSL = HandshakeLog
@@ -28,142 +31,6 @@ module CH = Parsers.ClientHello
 module SH = Parsers.RealServerHello
 module HRR = Parsers.HelloRetryRequest
 module FSH = Parsers.ServerHello
-
-// For readabililty, we try to open/abbreviate fewer modules
-
-(* A flag for runtime debugging of Handshake data.
-   The F* normalizer will erase debug prints at extraction
-   when this flag is set to false. *)
-val discard: bool -> ST unit
-  (requires (fun _ -> True))
-  (ensures (fun h0 _ h1 -> h0 == h1))
-let discard _ = ()
-let print s = discard (IO.debug_print_string ("HS | "^s^"\n"))
-unfold val trace: s:string -> ST unit
-  (requires (fun _ -> True))
-  (ensures (fun h0 _ h1 -> h0 == h1))
-unfold let trace = if DebugFlags.debug_HS then print else (fun _ -> ())
-
-// TODO : implement resumption
-//val getCachedSession: cfg:config -> ch:ch -> ST (option session)
-//  (requires (fun h -> True))
-//  (ensures (fun h0 i h1 -> True))
-//let getCachedSession cfg cg = None
-
-
-// *** internal stuff: state machine, reader/writer counters, etc.
-
-
-private
-let finishedId = HMAC_UFCMA.finishedId
-
-#set-options "--admit_smt_queries true"
-type machineState =
-  | C_init
-  | C_wait_ServerHello
-  | C13_wait_Finished1
-  | C13_sent_EOED:
-    digest ->
-    option HSM.certificateRequest13 ->
-    i:finishedId & cfk:KeySchedule.fink i -> machineState // TLS 1.3#20 aggravation
-  | C_wait_NST of bool           // server must send NewSessionticket
-  | C_wait_CCS of bool * digest  // TLS classic, resume & digest to be MACed by server
-  | C_wait_R_Finished1 of digest // TLS resume, digest to be MACed by server
-  | C_wait_ServerHelloDone     // TLS classic
-  | C_wait_Finished2 of digest // TLS classic, digest to be MACed by server
-  | C_Complete //19-06-07 to be split between 1.2 and 1.3
-
-  | S_Idle //19-06-07 may disappear
-  | S13_sent_ServerHello         // TLS 1.3, intermediate state to encryption
-  | S13_wait_EOED                // TLS 1.3, sometimes waiting for EOED
-  | S13_wait_Finished2 of digest // TLS 1.3, digest to be MACed by client
-  | S_wait_CCS1                  // TLS classic
-  | S_wait_Finished1 of digest // TLS classic, digest to the MACed by client
-  | S_wait_CCS2 of digest      // TLS resume (CCS)
-  | S_wait_CF2 of digest       // TLS resume (CF)
-  | S_Complete
-
-//17-03-24 consider using instead "if role = Client then clientState else serverServer"
-//17-03-24 but that may break extraction to Kremlin and complicate typechecking
-//17-03-24 we could also use two refinements.
-
-// Removed error states, consider adding again to ensure the machine is stuck?
-
-noeq type hs' = | HS:
-  #region: rgn {is_hs_rgn region} ->
-  r: role ->
-  nego: Nego.t region r ->
-  log: HandshakeLog.t {HandshakeLog.region_of log = region} ->
-  ks: KeySchedule.ks (*region*) ->
-  epochs: epochs region (Nego.nonce nego) ->
-  state: ref machineState {HS.frameOf state = region} -> // state machine; should be opaque and depend on r.
-  hs'
-
-let hs = hs' //17-04-08 around .fsti limitation
-
-let nonce (s:hs) = Nego.nonce s.nego
-let region_of (s:hs) = s.region
-let role_of (s:hs) = s.r
-let random_of (s:hs) = nonce s
-let config_of (s:hs) = Nego.local_config s.nego
-let version_of (s:hs) = Nego.version s.nego
-let get_mode (s:hs) = Nego.getMode s.nego
-let is_server_hrr (s:hs) = Nego.is_server_hrr s.nego
-let is_0rtt_offered (s:hs) =
-  let mode = get_mode s in Nego.zeroRTToffer mode.Nego.n_offer
-let is_post_handshake (s:hs) =
-  match !s.state with | C_Complete | S_Complete -> true | _ -> false
-let epochs_of (s:hs) = s.epochs
-
-(* WIP on the handshake invariant
-let inv (s:hs) (h:HS.mem) =
-  // let context = Negotiation.context h hs.nego in
-  let transcript = HandshakeLog.transcript h hs.log in
-  match HS.sel h s.state with
-  | C_wait_ServerHello ->
-      hs.role = Client /\
-      transcript = [clientHello hs.nonce offer] /\
-      "nego in Wait_ServerHello" /\
-      "ks in wait_ServerHello"
-  | _ -> True
-*)
-
-// the states of the HS sub-module will be subject to a joint invariant
-// for example the Nego state is a function of ours.
-
-
-let stateType (s:hs) = seq (epoch s.region (nonce s)) * machineState
-let stateT (s:hs) (h:HS.mem) : GTot (stateType s) = (logT s h, sel h s.state)
-
-let forall_epochs (s:hs) h (p:(epoch s.region (nonce s) -> Type)) =
-  (let es = logT s h in
-   forall (i:nat{i < Seq.length es}).{:pattern (Seq.index es i)} p (Seq.index es i))
-//epochs in h1 extends epochs in h0 by one
-
-(*
-#set-options "--admit_smt_queries true"
-let fresh_epoch h0 s h1 =
-  let es0 = logT s h0 in
-  let es1 = logT s h1 in
-  Seq.length es1 > 0 &&
-  es0 = Seq.slice es1 0 (Seq.length es1 - 1)
-
-(* vs modifies clauses? *)
-(* let unmodified_epochs s h0 h1 =  *)
-(*   forall_epochs s h0 (fun e ->  *)
-(*     let rs = regions e in  *)
-(*     (forall (r:rid{Set.mem r rs}).{:pattern (Set.mem r rs)} Map.sel h0 r = Map.sel h1 r)) *)
-*)
-
-let latest h (s:hs{Seq.length (logT s h) > 0}) = // accessing the latest epoch
-  let es = logT s h in
-  Seq.index es (Seq.length es - 1)
-
-// separation policy: the handshake mutates its private state,
-// only depends on it, and only extends the log with fresh epochs.
-
-// placeholder, to be implemented as a stateful property.
-let completed #rgn #nonce e = True
 
 // consider adding an optional (resume: option sid) on the client side
 // for now this bit is not explicitly authenticated.
@@ -178,81 +45,15 @@ let completed #rgn #nonce e = True
 // abstract invariant; depending only on the HS state (not the epochs state)
 // no need for an epoch states invariant here: the HS never modifies them
 
-assume val hs_invT : s:hs -> epochs:seq (epoch s.region (nonce s)) -> machineState -> Type0
-
-let hs_inv (s:hs) (h: HS.mem) = True
-(* 17-04-08 TODO deal with inferred logic qualifiers
-  hs_invT s (logT s h) (sel h (HS?.state s))  //An abstract invariant of HS-internal state
-  /\ Epochs.containsT s.epochs h                //Nothing deep about these next two, since they can always
-  /\ HS.contains s.state.ref ( h)                 //be recovered by 'recall'; carrying them in the invariant saves the trouble
-
-//A framing lemma with a very trivial proof, because of the way stateT abstracts the state-dependent parts
-*)
-
 #set-options "--admit_smt_queries true"
-let frame_iT_trivial  (s:hs) (rw:rw) (h0:HS.mem) (h1:HS.mem)
-  : Lemma (stateT s h0 = stateT s h1  ==>  iT s rw h0 = iT s rw h1)
-  = ()
-
-//Here's a framing on stateT connecting it to the region discipline
-let frame_stateT  (s:hs) (rw:rw) (h0:HS.mem) (h1:HS.mem) (mods:Set.set rid)
-  : Lemma
-    (requires
-      HS.modifies mods ( h0) ( h1) /\
-      HS.live_region h0 s.region /\
-      not (Set.mem s.region mods))
-    (ensures stateT s h0 = stateT s h1)
-  = ()
-
-//This is probably the framing lemma that a client of this module will want to use
-let frame_iT  (s:hs) (rw:rw) (h0:HS.mem) (h1:HS.mem) (mods:Set.set rid)
-  : Lemma
-    (requires
-      HS.modifies mods ( h0) ( h1) /\
-      HS.live_region h0 s.region /\
-      not (Set.mem s.region mods))
-    (ensures stateT s h0 = stateT s h1 /\ iT s rw h0 = iT s rw h1)
-=
-  frame_stateT s rw h0 h1 mods;
-  frame_iT_trivial s rw h0 h1
-
-
-
-// factored out; indexing to be reviewed
-val register: hs -> KeySchedule.recordInstance -> St unit
-let register hs keys =
-    let ep = //? we don't have a full index yet for the epoch; reuse the one for keys??
-      let h = Nego.Fresh ({ Nego.session_nego = None }) in
-      Epochs.recordInstanceToEpoch #hs.region #(nonce hs) h keys in // just coercion
-      // New Handshake does
-      // let KeySchedule.StAEInstance #id r w = keys in
-      // Epochs.recordInstanceToEpoch #hs.region #(nonce hs) h (Handshake.Secret.StAEInstance #id r w) in
-    Epochs.add_epoch hs.epochs ep // actually extending the epochs log
-
-val export: hs -> KeySchedule.exportKey -> St unit
-let export hs xk =
-  trace "exporting a key";
-  Monotonic.Seq.i_write_at_end hs.epochs.exporter xk
-
-let xkeys_of hs = Monotonic.Seq.i_read hs.epochs.exporter
-
-val map_ST2: 'c -> ('c -> 'a -> KeySchedule.ST0 'b) -> list 'a -> KeySchedule.ST0 (list 'b)
-let rec map_ST2 env f x = match x with
-  | [] -> []
-  | a::tl -> f env a :: map_ST2 env f tl
-
-let rec iutf8 (m:bytes) : St (s:string{String.length s < pow2 30 /\ utf8_encode s = m}) =
-    match iutf8_opt m with
-    | None -> trace ("Not a utf8 encoding of a string"); iutf8 m
-    | Some s -> s
 
 (* -------------------- Control Interface ---------------------- *)
 
 let create (parent:rid) cfg role =
   let r = new_region parent in
-  let log = HandshakeLog.create r None (* cfg.max_version (Nego.hashAlg nego) *) in
+  let log = HSL.create r None (* cfg.max_version (Nego.hashAlg nego) *) in
   //let nonce = Nonce.mkHelloRandom r r0 in //NS: should this really be Client?
-  let ks, nonce = KeySchedule.create #r role cfg.is_quic in
+  let ks, nonce = KS.create #r role cfg.is_quic in
   let nego = Nego.create r role cfg nonce in
   let epochs = Epochs.create r nonce in
   let state = ralloc r (if role = Client then C_init else S_Idle) in
@@ -265,7 +66,7 @@ let rekey s c = FStar.Error.unexpected "rekey: not yet implemented"
 
 let send_ticket hs app_data =
   if is_post_handshake hs then
-    let _ = server_Ticket hs app_data in true
+    let _ = server_Ticket13 hs app_data in true
   else false
 
 let request s c = FStar.Error.unexpected "request: not yet implemented"
@@ -286,11 +87,11 @@ let next_fragment_bounded (hs:hs) i (max:nat) =
     // after sending ServerHello in plaintext, we continue with encrypted traffic
     // otherwise, we just returns buffered messages and signals
     | HSL.Outgoing None None false, C_init ->
-      (match client_ClientHello hs i with
+      (match client_ClientHello hs with
       | Error z -> Error z
       | Correct () -> Correct(HSL.write_at_most hs.log i max))
     | HSL.Outgoing None None false, S13_sent_ServerHello ->
-      (match server_ServerFinished_13 hs i with
+      (match server_ServerFinished_13 hs with
       | Error z -> Error z
       | Correct () -> Correct(HSL.write_at_most hs.log i max))
     | HSL.Outgoing None None false, C13_sent_EOED d ocr cfk ->
